

第九次作业解答:

$$1. \text{解: } 15) \mathcal{L} \left\{ \frac{1}{b^2 - a^2} (\cos at - \sin bt) \right\} = \frac{1}{b^2 - a^2} \cdot \left(\frac{p}{p^2 + a^2} - \frac{b}{p^2 + b^2} \right)$$

$$19) \mathcal{L} \{ t e^{5t} \} = - \left(\frac{1}{p-5} \right)' = \frac{1}{(p-5)^2}$$

$$\begin{aligned} 112) \mathcal{L} \left\{ \frac{d^2}{dt^2} (e^{-at} \sin wt) \right\} &= p^2 \mathcal{L} [e^{-at} \sin wt] - p \cdot f'(0) - f'(0) \\ &= p^2 \cdot \frac{w}{(p+a)^2 + w^2} - w \end{aligned}$$

$$114) \mathcal{L} \left\{ \int_0^t t e^{2t} dt \right\} = \frac{\mathcal{L} \{ t e^{2t} \}}{p} = \frac{- \left(\frac{1}{p-2} \right)'}{p} = \frac{1}{p(p-2)^2}$$

$$\begin{aligned} 116) \mathcal{L} \left\{ \int_0^t (t-\tau)^n e^{-a\tau} \cos w\tau d\tau \right\} &= \mathcal{L} \{ t^n * e^{-at} \cos wt \} \\ &= \mathcal{L} \{ t^n \} \mathcal{L} \{ e^{-at} \cos wt \} \\ &= \frac{n!}{p^{n+1}} \cdot \frac{p+a}{(p+a)^2 + w^2} = \frac{n! (p+a)}{p^{n+1} ((p+a)^2 + w^2)} \end{aligned}$$

$$118) \mathcal{L} \{ \cos w(t-\varphi) h(t-2\varphi) \}$$

$$= \mathcal{L} \{ \cos w(t-2\varphi) + \varphi \} h(t-2\varphi)$$

$$= e^{-2p\varphi} \mathcal{L} \{ \cos w(t+\varphi) \}$$

$$= e^{-2p\varphi} \cdot \mathcal{L} \{ \cos wt \cdot \cos w\varphi - \sin wt \cdot \sin w\varphi \}$$

$$= e^{-2p\varphi} \cdot \left[\frac{p \cos w\varphi}{p^2 + w^2} - \frac{w \sin w\varphi}{p^2 + w^2} \right]$$

$$6. \text{解: } 12) \mathcal{L}^{-1} \left\{ \frac{1-p}{p^2 + p^2 + p + 1} \right\} = \mathcal{L}^{-1} \left\{ \frac{1}{p+1} - \frac{p}{p^2 + 1} \right\} = e^{-t} - \cos t$$

$$14) \mathcal{L}^{-1} \left\{ \frac{1}{p(p+a)} \right\} = \mathcal{L}^{-1} \left\{ \frac{1}{a} \left(\frac{1}{p} - \frac{1}{p+a} \right) \right\} = \frac{1}{a} (1 - e^{-at})$$

$$16) \mathcal{L}^{-1} \left\{ \frac{1}{(p^2+1)(p^2+3)} \right\} = \mathcal{L}^{-1} \left\{ \frac{1}{2} \left(\frac{1}{p^2+1} - \frac{1}{p^2+3} \right) \right\} = \frac{1}{2} (\sin t - \frac{1}{\sqrt{3}} \sin \sqrt{3} t)$$

$$18) \mathcal{L}^{-1} \left\{ \frac{1}{p(p-2)^2} \right\} = \mathcal{L}^{-1} \left\{ \frac{1}{4p} - \frac{1}{4(p-2)} + \frac{1}{2(p-2)^2} \right\} = \frac{1}{4} (1 - e^{2t} + 2te^{2t})$$



$$(12) \mathcal{L}^{-1}\left\{\frac{a^2 p}{p^4 + a^4}\right\} = \mathcal{L}^{-1}\left\{\frac{p}{p^4 + 4\left(\frac{a}{\sqrt{2}}\right)^4}\right\} = a^2 \cdot \frac{1}{2 \cdot \left(\frac{a}{\sqrt{2}}\right)^2} \left(\sin \frac{a}{\sqrt{2}} t\right) \left(\operatorname{sh} \frac{a}{\sqrt{2}} t\right) = \left(\sin \frac{a}{\sqrt{2}} t\right) \left(\operatorname{sh} \frac{a}{\sqrt{2}} t\right)$$

(Pig 页表格中, $\frac{1}{p^4 + a^4} \sim \frac{1}{2a^2} \sin at \operatorname{sh} at$)

$$(18) \mathcal{L}^{-1}\left\{\frac{1-p}{(p+1)(p+1)} e^{-10p}\right\} = \mathcal{L}^{-1}\left\{e^{-10p} \left(\frac{1}{p+1} - \frac{p}{p^2+1}\right)\right\} = (e^{-(t+10)} - \cos(t-10)) h(t+10)$$

7. 解: (3) 设 $\mathcal{L}(y(t)) = Y(p)$. 则 $\mathcal{L}\{y''(t)\} = p^2 Y - p y(0) - y'(0) = p^2 Y - 1$

$$\mathcal{L}\{y'(t)\} = pY - y(0) = pY$$

\therefore 对原方程两边作拉氏变换:

$$(p^2 Y - 1) - (a+b)pY + abY = 0. \Rightarrow Y = \frac{1}{(p-a)(p-b)}$$

$$\therefore y(t) = \mathcal{L}^{-1}\left\{\frac{1}{(p-a)(p-b)}\right\} = \frac{1}{b-a} (e^{at} - e^{bt})$$

(5) 设 $\mathcal{L}(y(t)) = Y(p)$. 则 $\mathcal{L}\{y''(t)\} = p^2 Y - p y(0) - y'(0) = p^2 Y + p + 2$

$$\mathcal{L}\{\sin t\} = \frac{1}{p^2+1}, \quad \mathcal{L}\{5\cos 2t\} = \frac{5p}{p^2+4}$$

\therefore 对原方程两边作拉氏变换:

$$(p^2 Y + p + 2) - Y = \frac{1}{p^2+1} + \frac{5p}{p^2+4} \Rightarrow Y = -\frac{p^2 + p^2 + p + 8}{(p^2+1)(p^2+4)} = -\left(\frac{2}{p^2+1} + \frac{p}{p^2+4}\right)$$

$$\therefore y(t) = \mathcal{L}^{-1}\left\{-\left(\frac{2}{p^2+1} + \frac{p}{p^2+4}\right)\right\} = -2\cos t - 2\sin t$$

(10) 设 $\mathcal{L}\{x(t)\} = X(p)$. $\Rightarrow Y(p), Z(p)$ 同解.

$$\text{则 } \mathcal{L}\{x'(t)\} = pX, \quad \mathcal{L}\{y'(t)\} = pY, \quad \mathcal{L}\{z'(t)\} = pZ, \quad \mathcal{L}\{t\} = \frac{1}{p^2}$$

$$\therefore \begin{cases} pX - pY = 0 \\ pY + pZ = \frac{1}{p^2} \\ pX - pZ = \frac{1}{p^2} \end{cases} \Rightarrow \begin{cases} X = \frac{1}{2p^2} + \frac{1}{2p^2} \\ Y = \frac{1}{2p^2} + \frac{1}{2p^2} \\ Z = \frac{1}{2p^2} - \frac{1}{2p^2} \end{cases} \Rightarrow \begin{cases} x(t) = \frac{1}{2}t + \frac{t^2}{4} \\ y(t) = \frac{1}{2}t + \frac{t^2}{4} \\ z(t) = \frac{1}{2}t - \frac{t^2}{4} \end{cases}$$

(8). 同法设.

$$\begin{cases} pY - a + pX - b = 4Y + \frac{1}{p} \\ pY - a + X = 3Y + \frac{2}{p^2} \end{cases} \Rightarrow \begin{cases} X = \frac{1}{p^2} + \frac{3}{2} \frac{1}{p^2} + \frac{1}{4p} + \frac{(b-a)}{p-2} + \frac{(a-b)}{(p-2)^2} \\ Y = \frac{1}{2p^2} + \frac{1}{4p} + \frac{(a-b)}{p-2} + \frac{(a-b)}{(p-2)^2} \end{cases} \Rightarrow \begin{cases} x(t) = t^2 + \frac{3}{2}t + \frac{1}{4} + (b-a)e^{2t} + (a-b)t e^{2t} \\ y(t) = \frac{1}{2}t + \frac{1}{4} + (a-b)e^{2t} + (a-b)t e^{2t} \end{cases}$$

